#+TITLE: Incremental Correctness (Induction)
#+TAGS: proof induction computer-science
#+OPTIONS: \n:t


#+begin_quote
Increment(y):
    if  =y = 0= then =return(1)= else
        if =(y mod 2) == 1= then
            return =(2 Â· Increment(y/2))=
        else =return (y + 1)=
#+end_quote

/Solution:/

1. Base case =n=0=
  Clearly if n=0 then =Increment(0)= returns 1.

2. Assume true for all =n<y= prove for =n = y + 1=
   When n is even, ie. =n=2k= then.
  #+begin_quote
Increment(2k) \\
    =2k mod 2 == 0 =>= return =2k + 1=
  #+end_quote

  If n is odd such that =n = 2m + 1=
=(2m + 1 mod 2) = 1= \\
then
\begin{equation}
\begin{aligned}
2 . increment([2m+1]/2) =& 2 . increment([m + 1/2]) \\
 =& 2. increment(m) \\
 =& 2(2m+1) \\
 =& 2m+2 = y + 1 \\
 \qed
\end{aligned}
\end{equation}
