#+TITLE: Factorial_formulae
* Problem
Prove that
\begin{equation}
\sum_{i=0}^n i \times i! = (n + 1)! - 1
\end{equation}

by induction.

** Solution

When n = 0

\begin{align}
LHS &= \sum_{i=0}^0 i \times i \\
&= 0 \times 0! = 0 \\
\end{align}
and
\begin{align}
RHS &= (0 + 1)! - 1 \\
    &= 1! - 1 = 0
\end{align}

Assume this holds for n = y, prove for n = y + 1.

\begin{align}
LHS =& \sum_{i=0}^{y+1} i \times i! \\
=& \sum_{i=0}^y i \times i! + [y + 1 \times (y+1)!] \\
\end{align}
by assumption
\begin{align}
(y + 1)! - 1 + (y + 1) \times (y+1)! \\
(y+1)! \times ( 1 + y + 1 ) - 1 \\
(y+1)! \times (y + 2) - 1 \\
(y+2)! - 1 \\
\blacksquare
\end{align}
